src/Utils.v
@@ -99,19 +99,19 @@ Definition try_map {A B : Type} (f : A -> option B) (l : seq A) : option (seq B)
 
 Lemma try_map_map_distribute {A B C : Type} (f : B -> option C) (g : A -> B) l
   : try_map f (map g l) = try_map (fun x => f (g x)) l.
-Proof.
+Proof using .
   elim: l => //=.
   intros; by rewrite H.
 Qed.
 
 Lemma omap_some {A B} (e' : B) (f : A -> B) me : Some e' = omap f me -> exists e, me = Some e.
-Proof.
+Proof using .
   case: me => //=; eauto.
 Qed.
 
 Lemma omap_some' {A B} (e' : B) (f : A -> B) me
   : Some e' = omap f me -> exists e, Some e' = omap f (Some e).
-Proof.
+Proof using .
   move => someeq.
   suff: exists e, me = Some e.
   move: someeq.
@@ -119,4 +119,65 @@ Proof.
   case => e ->.
   eauto.
   apply: omap_some; eauto.
+Qed.
+
+ (*Todo: whichs more useful?*)
+(*Definition nth_level {A} l n : option A :=
+  if n <= size l then List.nth_error l (size l - n.+1) else None.*)
+Definition nth_level {A} a l n : A :=
+  if n < size l then nth a l (size l - n.+1) else a.
+Definition is_nth_level {A:eqType} (l : seq A) n x : bool :=
+   (n < size l) && (List.nth_error l (size l - n.+1) == Some x).
+
+Lemma is_nth_level_to_fn {A:eqType} a (l : seq A) n x
+  : is_nth_level l n x -> (nth_level a l n == x).
+Proof using .
+  unfold nth_level; unfold is_nth_level.
+  case: (n < size l); simpl; auto.
+  generalize (size l - n.+1) as y.
+  move => y; move: y l.
+  elim; intros until l; case: l; simpl; auto.
+Qed.
+
+Lemma fn_to_is_nth_level {A:eqType} a (l : seq A) n x
+  : n < size l -> is_nth_level l n x = (nth_level a l n == x).
+Proof using .
+  unfold nth_level; unfold is_nth_level.
+  move => nlt.
+  rewrite nlt; simpl.
+  suff: (size l - n.+1 < size l).
+  generalize (size l - n.+1) => y.
+  clear nlt.
+  elim: y l; intros until l; case: l; easy.
+  move: nlt. generalize (size l) as sz.
+  case; try easy.  
+  intros.
+  rewrite subSS.
+  by apply sub_ord_proof.
+Qed.
+
+Lemma ListIn_in {A:eqType} (x : A) l : List.In x l -> x\in l.
+Proof using .
+  elim: l => //=.
+  move => a l IH.
+  rewrite in_cons.
+  case.
+  - move ->; apply /orP.
+    left; by apply /eqP.
+  - move /IH => IH'; apply /orP; by right.
+Qed.
+
+Lemma is_nth_level_in  {A:eqType} (l : seq A) n x
+  : is_nth_level l n x -> x \in l.
+Proof using .
+  unfold is_nth_level; case /andP => _.
+  generalize (size l - n) as m.
+  move => m.
+  elim: m l.
+  - case; simpl; auto.
+    move => a l.
+    move /eqP => H.
+    apply List.nth_error_In in H.
+    by apply ListIn_in.
+  - move => m IH; case; simpl; auto; intro_to is_true.
 Qed.
